# Fold Left vs. Fold Right

Having built both `fold_right` and `fold_left`, it's worthwhile to
compare and contrast them.  The immediately obvious difference is
the order in which they combine elements from the list:  right to left
vs. left to right.  When the operator being used to combine elements
is *associative*, that order doesn't doesn't change the final value of
the computation.  But for non-associative operators like `(-)`, it can:
```
# List.fold_right (-) [1;2;3] 0;;  (* 1 - (2 - (3 - 0)) *)
- : int = 2
# List.fold_left (-) 0 [1;2;3];;   (* ((0 - 1) - 2) - 3 *)
- : int = -6 
```

A second difference is that `fold_left` is tail recursive whereas `fold_right` is
not. So if you need to use `fold_right` on a very lengthy list, you may
instead want to reverse the list first then use `fold_left`; the operator
will need to take its arguments in the reverse order, too:
```
# List.fold_right (fun x y -> x - y) [1;2;3] 0;;
- : int = 2

# List.fold_left (fun y x -> x - y) 0 (List.rev [1;2;3]);;
- : int = 2

# List.fold_left (fun x y -> y - x) 0 (List.rev (0--1_000_000));;
- : int = 500000  

# List.fold_right (fun y x -> x - y) (0--1_000_000) 0;;
Stack overflow during evaluation (looping recursion?)
```
Of course we could have written `fun x y -> x - y` as `(-)` in the code above,
but we didn't in this one case just so you could see how the argument order has to change.
Recall that `x--y` tail-recursively computes the list containing all the
integers from `x` to `y` inclusive:
```
let (--) i j =
  let rec from i j l =
    if i>j then l
    else from i (j-1) (j::l)
    in from i j []
```

We could even define a tail-recursive version of `fold_right` by baking in the list
reversal:
```
let fold_right_tr f l accu =
  List.fold_left (fun acc elt -> f elt acc) accu (List.rev l)

# fold_right_tr (fun x y -> x - y) (0--1_000_000) 0;;
- : int = 500000 
```

A third difference is the types of the functions.  It can be hard to remember
what those types are!  Luckily we can always ask the toplevel:
```
# List.fold_left;;
- : ('a -> 'b -> 'a) -> 'a -> 'b list -> 'a = <fun>

# List.fold_right;;
- : ('a -> 'b -> 'b) -> 'a list -> 'b -> 'b = <fun>
```

To understand those types, look for the list argument in each one of them.  That tells
you the type of the values in the list.  Then look for the type of the return value; 
that tells you the type of the accumulator.  From there you can work out everything else.

* In `fold_left`, the list argument is of type `'b list`, so the list
  contains values of type `'b`.  The return type is `'a`, so the
  accumulator has type `'a`.  Knowing that, we can figure out that the
  second argument is the initial value of the accumulator (because it has
  type `'a`).  And we can figure out that the first argument, the
  combining operator, takes as its own first argument an accumulator value
  (because it has type `'a`), as its own second argument a list element
  (because it has type `'b`), and returns a new accumulator value.
  
* In `fold_right`, the list argument is of type `'a list`, so the list
  contains values of type `'a`.  The return type is `'b`, so the
  accumulator has type `'b`.  Knowing that, we can figure out that the
  third argument is the initial value of the accumulator (because it has
  type `'b`).  And we can figure out that the first argument, the
  combining operator, takes as its own second argument an accumulator value
  (because it has type `'b`), as its own first argument a list element
  (because it has type `'a`), and returns a new accumulator value.

You might wonder why the argument orders are different between the two `fold`
functions.  I have no good answer to that question.  Other libraries 
do in fact use different argument orders.

If you find it hard to keep track of all these argument orders, the
[`ListLabels` module][listlabels] in the standard library can help.  It uses labeled
arguments to give names to the combining operator (which it calls `f`)
and the initial accumulator value (which it calls `init`).  Internally,
the implementation is actually identical to the `List` module.
```
# ListLabels.fold_left;;
- : f:('a -> 'b -> 'a) -> init:'a -> 'b list -> 'a = <fun>

# ListLabels.fold_right;;
- : f:('a -> 'b -> 'b) -> 'a list -> init:'b -> 'b = <fun>

# ListLabels.fold_left ~f:(fun x y -> x - y) ~init:0 [1;2;3];;
- : int = -6

# ListLabels.fold_right ~f:(fun y x -> x - y) ~init:0 [1;2;3];;
- : int = -6
```

Notice how in the two applications of fold above, we are able to write the arguments
in a uniform order thanks to their labels.  However, we still have to be careful
about which argument to the combining operator is the list element vs. the accumulator value.

[listlabels]: http://caml.inria.fr/pub/docs/manual-ocaml/libref/ListLabels.html

* * *
<i>
**A digression on labeled arguments and fold**

It's possible to write our own version of the fold functions that would
label the arguments to the combining operator, so we don't even have to remember
their order:
```
let rec fold_left ~op:(f: acc:'a -> elt:'b -> 'a) ~init:accu l =
  match l with
    [] -> accu
  | a::l -> fold_left ~op:f ~init:(f ~acc:accu ~elt:a) l 

let rec fold_right ~op:(f: elt:'a -> acc:'b -> 'b) l ~init:accu =
  match l with
    [] -> accu
  | a::l -> f ~elt:a ~acc:(fold_right ~op:f l ~init:accu)
```
But those functions aren't as useful as they might seem:
```
# fold_left ~op:(+) ~init:0 [1;2;3];;
Error: This expression has type int -> int -> int                                      
but an expression was expected of type acc:'a -> elt:'b -> 'a
```
The problem is that the built-in `(+)` operator doesn't have labeled arguments,
so we can't pass it in as the combining operator to our labeled functions.
We'd have to define our own labeled version of it:
```
# let add ~acc ~elt = acc+elt;;
val add : acc:int -> elt:int -> int = <fun>

# fold_left ~op:add ~init:0 [1;2;3];;
- : int = 6 
``` 
But now we have to remember that the `~acc` parameter to `add` will become
the left-hand argument to `(+)`.  That's not really much of an improvement
over what we had to remember to begin with.

</i>
* * *
